%!TEX root =  main.tex
\chapter*{Chapter 7}
\label{sec:7}

\noindent\textbf{7.1}

    \begin{enumerate}[(a)]
    \item
    \begin{align*}
    P &=(\hat{\mu}-\mu\ge\sqrt{\dfrac{2log(1/\delta)}{T}})\\
    &=\sum^{\infty}_{n=1}E[\{T=n\}\|\{\hat{\mu}-\mu\ge\sqrt{\dfrac{2log(1/\delta)}{T}}\}]\\
    &=\sum^{\infty}_{n=1}E[\|\{T=n\}\delta]\\
    &=\delta\sum^{\infty}_{n=1}P(T=n)\\
    &=\delta
    \end{align*}

    \item
    $\hat{\mu}-\mu=\frac{1}{n}\sum^{\infty}_{t=1}(X_t-\mu)\ge\sqrt{\dfrac{2-\log(1/\delta)}{T}}$

    T=min(n)

    $E_t=\|\{T=t\}$ is $\mathcal{F}_t$-measurable

    \item
    \begin{align*}
    P(\hat{\mu}-\mu\ge\sqrt{\dfrac{2log(T(T+1)/\delta}{T}}) &\le P(\bigcup^{\infty}_{n=1}\hat{\mu}-\mu\ge\sqrt{\dfrac{2log(n(n+1)/\delta}{n}})\\
    &\le \sum^{\infty}_{n=1}P(\hat{\mu}-\mu\ge\sqrt{\dfrac{2log(n(n+1)/\delta}{n}})\\
    &\le \sum^{\infty}_{n=1} \dfrac{\delta}{n(n+1)}\\
    &\le \delta
    \end{align*}



\noindent\textbf{7.3}
    $E[Ti(n)]\le\dfrac{-8ln\delta}{\bigtriangleup_i}+\delta n(n=1)$


    $R_n=E[\overline{R_n}]\le\sum^{k}_{i=2}\dfrac{-8ln\delta}{\bigtriangleup_i}+\bigtriangleup_i\delta n(n+1)$


    Choosing
    $\delta=\dfrac{\sum^{k}_{i=2}\frac{8}{\bigtriangleup_i}}{\sum^{k}_{i=2}\bigtriangleup_i   n(n+1)}$
    \begin{align*}
    R_n &\le\sum^{k}_{i=2}\frac{8}{\bigtriangleup_i}+\sum^{k}_{i=2}\frac{8}{\bigtriangleup_i}ln\frac{\sum^{k}_{i=2}\bigtriangleup_i n(n+1)}{\sum^{k}_{i=2}\frac{8}{\bigtriangleup_i}}\\
    &:=h(n,k)
    \end{align*}
    $g(n,k,\delta)=\dfrac{\sqrt{h(n,k)}}{\delta};f(n,k)=\sqrt{h(n,k)}$
    \begin{align*}
    P(\overline{R_n}\ge g(n,k,\delta)) &\le\dfrac{R_n}{g(n,k,\delta)}\\
    &\le\dfrac{h(n,k)}{g(n,k,\delta)}\\
    &=\dfrac{h(n,k)}{\sqrt{h(n,k)}}\delta\\
    &=\sqrt{h(n,k)}\delta\\
    &=f(n,k)\delta
    \end{align*}


\noindent\textbf{7.6}
    \item
    \begin{align*}
    \hat{\delta}^2 &=\frac{1}{n}\sum^{n}_{t=1}(\hat{\mu}-X_t)^2\\
    &=\frac{1}{n}\sum^{n}_{t=1}[(\hat{\mu}-\mu)+(\mu-X_t)]^2\\
    &=\frac{1}{n}\sum^{n}_{t=1}(\hat{\mu}-\mu)^2+\frac{1}{n}\sum^{n}_{t=1}(\mu-X-t)^2+\frac{2}{n}\sum^{n}_{t=1}(\hat{\mu}-\mu)(\mu-X_t)
    \end{align*}
    $\because\hat{\mu}-\mu=\frac{1}{n}\sum^{n}_{t=1}X_t-\mu=\frac{1}{n}\sum^{n}_{t=1}(X_t-\mu)$
    \begin{align*}
    \therefore\frac{2}{n}\sum^{n}_{t=1}(\hat{\mu}-\mu)(\mu-X-t) &=\frac{2}{n}\sum^{n}_{t=1}[\frac{1}{n}\sum^{n}_{t=1}(X_t-\mu)](\mu-X_t)\\
    &=-2[\frac{1}{n}\sum^{n}_{t=1}(X_t-\mu)]^2\\
    &=-2[\hat{\mu}-\mu]^2
    \end{align*}
    \begin{align*}
    \hat{\delta}^2 &=(\hat{\mu}-\mu)^2+\frac{1}{n}\sum^{n}_{t=1}(\mu-X_t)^2-2(\hat{\mu}-\mu)^2\\
    &=\frac{1}{n}\sum^{n}_{t=1}(\mu-X_t)^2-(\hat{\mu}-\mu)^2
    \end{align*}
    
    